MY PRIMES!

src/newprimes.lean
@@ -4,8 +4,7 @@ import tactic
 open nat
 
 def divisors_aux (n : ℕ) : ℕ → list ℕ
-| 0     := [1]
-| 1     := [1]
+| 0     := []
 | (h+1) := if n % h = 0
            then [h] ++ divisors_aux h
            else divisors_aux h
@@ -18,34 +17,139 @@ def is_in_list (n : ℕ) : list ℕ → bool
 
 #eval divisors 5
 #eval divisors 4
+#eval divisors_aux 12 13
+#eval divisors_aux 0 10
+#eval divisors 0
+#eval divisors_aux 12 1
+#eval divisors_aux 12 0
 
-def myprime (p : ℕ) : Prop := (p ≥ 2) ∧ divisors p = [1,p]
+def myprime (p : ℕ) : Prop := (p ≥ 2) ∧ divisors p = [p,1]
 
-lemma h_div_in_list (p a : ℕ) (h : a <= p) (j : 1 <= a) : prime p → divisors_aux p a = [1] :=
+example (n : ℕ) : divisors_aux n 0 = [] := rfl
+
+lemma def_aux (h n : ℕ) : divisors_aux n (h+1) = if n % h = 0
+                                            then [h] ++ divisors_aux n h
+                                            else divisors_aux n h := rfl
+
+lemma ite_zero_eq_zero (p : ℕ) : ite (0 = 0) ([p] ++ divisors_aux p p) (divisors_aux p p) =
+  ([p] ++ (divisors_aux p p)) := rfl
+
+lemma mod_one (n : ℕ) (h : n ≠ 0) : divisors_aux n 1 = [] :=
 begin
-  induction a,
+  rw def_aux,
+  have o₀ : n % 0 = n, from mod_def n 0,
+  have o₁ : n % 0 ≠ 0, from ne_of_eq_of_ne o₀ h,
+  have o₂ : ite (n % 0 = 0) ([0] ++ divisors_aux n 0) (divisors_aux n 0)
+    = divisors_aux n 0, from if_neg o₁,
+  rw o₂,
+  refl,
+end
+
+lemma ffa (p q : ℕ) (h₁ : q = p) (h₂ : q < p): false :=
+begin
+  rw h₁ at h₂,
+  revert h₂,
+  contrapose,
+  intro,
+  exact irrefl p,
+end
+
+lemma ffs (p q : ℕ) (h₁ : q = p) : ¬(q < p) := λ a, ffa p q h₁ a
+
+lemma ffss (p q : ℕ) (h₁ : q < p) : ¬(q = p) := λ a, ffa p q a h₁
+
+lemma prime_mod (p b : ℕ) (h₁ : prime p) (h₂ : 2 ≤ b) (h₃ : b < p) : p % b ≠ 0 :=
+begin
+  have o₁ : p % b = 0 → b ∣ p, from dvd_of_mod_eq_zero,
+  have o₂ : ¬(b ∣ p) → ¬(p % b = 0), from mt o₁,
+  apply o₂,
+  have o₃ : 2 ≤ p ∧ ∀ (m : ℕ), m ∣ p → m = 1 ∨ m = p, from h₁,
+  have o₄ : ∀ (m : ℕ), m ∣ p → m = 1 ∨ m = p, from o₃.right,
+  have o₅ : b ∣ p → b = 1 ∨ b = p, from o₄ b,
+  have o₆ : ¬(b = 1 ∨ b = p) → ¬(b ∣ p), from mt (o₄ b),
+  have o₇ : ¬(b = 1) ∧ ¬(b = p) → ¬(b = 1 ∨ b = p), from not_or_distrib.mpr,
+  have o₈ : ¬(b = 1) ∧ ¬(b = p) → ¬(b ∣ p), from λ a, o₆ (o₇ a),
+  have o₉ : ¬(b = 1), from λ a, ffa b 1 a.symm h₂,
+  have s₁ : ¬(b = p), from ffss p b h₃,
+  exact o₈ ⟨o₉,s₁⟩,
+end
+
+lemma Reid_B (a p : ℕ) (h₁ : 2 <= a) (h₂ : a <= p) (h₃ : prime p)
+  : divisors_aux p a = [1] :=
+begin
+  induction h₁,
   {
-    intro,
+    rw def_aux,
+    have o₀ : p % 1 = 0, from mod_one p,
+    have o₁ : ite (p % 1 = 0) ([1] ++ divisors_aux p 1) (divisors_aux p 1)
+      = [1] ++ divisors_aux p 1, from if_pos o₀,
+    rw o₁,
+    have o₂ : p ≠ 0, from prime.ne_zero h₃,
+    have o₃ : divisors_aux p 1 = [], from mod_one p o₂,
+    rw o₃,
     refl,
   },
   {
-    intro,
-    tidy,
-  },
+    rw def_aux,
+    have o₃ : h₁_b < p, from h₂,
+    have o₄ : h₁_b ≤ p, from le_of_lt h₂,
+    rw h₁_ih o₄,
+    have o₅ : p % h₁_b ≠ 0, from prime_mod p h₁_b h₃ h₁_a h₂,
+    exact if_neg o₅,
+  }
 end
 
 lemma my_prime_good (p n : ℕ) : prime p → myprime p :=
 have s₁ : prime p → (p ≥ 2), from prime.two_le,
+have s₆ : prime p → p ≠ 1, from prime.ne_one,
 have s₄ : prime p → (n ∣ p → n = 1 ∨ n = p), from λ (pp : prime p), (dvd_prime pp).mp,
-have s₂ : (n ∣ p → n = 1 ∨ n = p) → divisors p = [1,p], from
+have s₅ : prime p → divisors_aux p p = [1], from
 begin
   intro,
-  sorry
+  refine Reid_B p p _ _ a,
+  {exact s₁ a},
+  {refl},
 end,
-have s₃ : (p ≥ 2) ∧ (divisors p = [1,p]) → myprime p, from
+have s₂ : prime p → divisors p = [p,1], from
+begin
+  intro,
+  unfold divisors,
+  rw [def_aux, mod_self p, ite_zero_eq_zero, s₅],
+  refl,
+  exact a
+end,
+have s₃ : (p ≥ 2) ∧ (divisors p = [p,1]) → myprime p, from
   begin intros, unfold myprime, assumption, end,
 show prime p → myprime p, from
 begin intro, apply s₃, split,
   exact s₁ a,
-  exact s₂ (s₄ a)
+  exact s₂ a
+end
+
+lemma p_mod_p_ite (p : ℕ) : ite (p % p = 0) ([p] ++ divisors_aux p p) (divisors_aux p p)
+  = [p] ++ divisors_aux p p :=
+begin
+  have o₁ : p % p = 0, from mod_self p,
+  exact if_pos o₁,
+end
+
+lemma good_prime_my (p : ℕ) : myprime p → prime p :=
+λ b,
+begin
+  have s₁ : (p ≥ 2), from b.left,
+  have s₂ : divisors p = [p,1] → (∀ n : ℕ, n ∣ p → n = 1 ∨ n = p), from
+  begin
+    unfold divisors,
+    rw def_aux,
+    rw p_mod_p_ite,
+    intros,
+    sorry, --Think about how to do this proof (break into peices)
+  end,
+  have s₃ : divisors p = [p,1], from b.right,
+  have s₄ : (∀ n : ℕ, n ∣ p → n = 1 ∨ n = p), from s₂ s₃,
+  show prime p, from
+  begin
+    unfold prime,
+    exact ⟨s₁, s₂ s₃⟩,
+  end,
 end
