src/cram.lean
@@ -1,129 +1,29 @@
 import tactic.suggest
 import tactic.solve_by_elim
 import data.nat.basic
+import data.nat.prime
 
 open tactic
 open nat
 
 namespace tactic
 
-meta def cram_old (discharger : tactic unit := done) : tactic string :=
-(suggest_core discharger).mfirst
-  (λ a : suggest.application,
-    do guard (a.num_goals = 0 ∨ a.num_goals = 1),
-       write a.state,
-       return a.script)
-
-meta def cram' (discharger : tactic unit := done) : tactic string :=
-(suggest_core discharger).mfirst
-  (λ a : suggest.application,
-    do guard (a.num_goals = 0 ∨ a.num_goals = 1),
-       if a.num_goals = 0 then do write a.state, return a.script
-       else if a.num_goals = 1 then do write a.state, script ← library_search, return script
-       else fail "")
-
-meta def cram (discharger : tactic unit := done) : tactic string :=
-(suggest_core discharger).mfirst
-  (λ a : suggest.application,
-    do guard (a.num_goals = 1), write a.state, script ← library_search, return script)
-
--- want to filter this mllist so that we only have the results with num_goals = 1.
--- want recurse on cram so that to some depth, and if the goal is solved return the message
--- just like library_search.
-
-open suggest
-
-meta def solve_by_suggest_aux (discharger : tactic unit)
-  (asms : tactic (list expr))
-  (g : expr) : ℕ → tactic unit
-| 0 := do trace (tactic_statement g)
-| (n+1) := do (do done, [g] ← get_goals <|> fail "FAIL!!!", trace (tactic_statement g))
-              <|>
-              (apply_assumption asms $ solve_by_suggest_aux n) <|>
-              (discharger >> solve_by_suggest_aux n)
-
-meta structure by_suggest_opt :=
-  (all_goals : bool := ff)
-  (discharger : tactic unit := done)
-  (assumptions : tactic (list expr) := mk_assumption_set false [] [])
-  (max_rep : ℕ := 3)
-
-meta def solve_by_suggest (opt : by_elim_opt := { }) : tactic unit :=
-do
-  [g] ← get_goals <|> fail "FAIL!!!",
-  tactic.fail_if_no_goals,
-  (if opt.all_goals then id else focus1) $
-    solve_by_suggest_aux opt.discharger opt.assumptions g opt.max_rep
-
-open interactive lean.parser interactive.types
-local postfix `?`:9001 := optional
+meta def cram : ℕ → tactic unit
+| 0     := done <|> all_goals tactic.interactive.library_search
+| (n+1) := done <|> all_goals (tactic.interactive.library_search >> cram n)
 
 namespace interactive
 
-meta def cram (discharger : tactic unit := done) : tactic unit :=
-tactic.cram >>= trace
-
---TODO
---*get baby_back to print all possible refine statements
---*Some major refactoring including suggest and solve_by_elim
-
---This tactic is suppose to be a mix between suggest and solve_by_elim.
---Solve_by_elim already works, just need it too print
-meta def baby_back (all_goals : parse $ (tk "*")?)
- (no_dflt : parse only_flag)
- (hs : parse simp_arg_list)
- (attr_names : parse with_ident_list)
- (opt : by_elim_opt := { }) : tactic unit :=
-
---duplicate code
-do [g] ← get_goals <|> fail "FAIL!",
-
-   asms ← mk_assumption_set no_dflt hs attr_names,
-   tactic.solve_by_elim { all_goals := all_goals.is_some, discharger := skip, assumptions := return asms, ..opt },
-
-   --s ← read,
-   trace (tactic_statement g)
-
-
-meta def solve_by_suggest (all_goals : parse $ (tk "*")?)
- (no_dflt : parse only_flag)
- (hs : parse simp_arg_list)
- (attr_names : parse with_ident_list)
- (opt : by_elim_opt := { }) : tactic unit :=
- do asms ← mk_assumption_set no_dflt hs attr_names,
-   tactic.solve_by_suggest { all_goals := all_goals.is_some, discharger := skip, assumptions := return asms, ..opt }
+meta def cram : tactic unit :=
+tactic.cram 10000
 
 end interactive
 
 end tactic
 
-example (a b c :ℕ) (h : a = b) (j : b < c) : a < c :=
+open nat
+
+example (n : ℕ) : ∃ a : ℕ, a > n ∧ prime (a-1) ∧ prime (a+1) :=
 begin
-  rw h,
-  exact j,
+  sorry
 end
-
-variables {m n k : ℕ}
-
-theorem lt_of_sub_lt_sub_left : m - n < m - k → k < n :=
-lt_imp_lt_of_le_imp_le (nat.sub_le_sub_left _)
-
-example : m - n < m - k → k < n :=
-begin solve_by_elim [lt_imp_lt_of_le_imp_le, nat.sub_le_sub_left], end
-
-example : m - n < m - k → k < n :=
-begin baby_back [lt_imp_lt_of_le_imp_le, nat.sub_le_sub_left], end
-
-example {m : nat} : max 0 m = m :=
-begin baby_back end
---max_eq_right (zero_le _)
-
-example {a b : ℕ} : a < b + 1 ↔ a ≤ b :=
-begin baby_back [nat.lt_succ_iff, lt_imp_lt_of_le_imp_le, nat.sub_le_sub_left] end
-
-example {a : ℕ} (h : a ≤ a / 2) : a = 0 :=
-begin baby_back [eq_zero_of_le_div, le_refl] end
---eq_zero_of_le_div (le_refl _) h
-
-example {a : ℕ} (h : a ≤ a / 2) : a = 0 :=
-begin suggest, solve_by_suggest [le_refl] end
